% NOTE DUPLICATE 439
% Operators dump: \odot$ \quad $\oplus$ \quad $\otimes$ \quad $\ominus$ \quad $\oslash
\documentclass[a4paper]{article}

%% Language and font encodings
\usepackage[english]{babel}
\usepackage[utf8x]{inputenc}
\usepackage[T1]{fontenc}

%% Sets page size and margins
\usepackage[a4paper,top=1.25cm,bottom=1.25cm,left=1.0cm,right=1.0cm,marginparwidth=1.25cm]{geometry}

%% Useful packages
\usepackage{amsmath}
\usepackage{graphicx} 
\usepackage[colorinlistoftodos]{todonotes}
\usepackage[colorlinks=true, allcolors=blue]{hyperref}
\DeclareMathSizes{12}{30}{16}{12}
\usepackage[final]{pdfpages}
\usepackage{gensymb}
\usepackage{empheq}
\usepackage[section]{placeins}
\usepackage[most]{tcolorbox}
\usepackage{esint}
\usepackage{amssymb}
\usepackage{centernot}
\usepackage{multicol}
\usepackage{etoolbox}
\usepackage{xparse}
\usepackage{xcolor} % black, blue, brown, cyan, darkgray, gray, green, lightgray, lime, magenta, olive, orange, pink, purple, red, teal, violet, white, yellow.
\usepackage{soul}
\delimitershortfall-1sp
\usepackage{mleftright}
\mleftright
\def\ml{\mleft}
\def\mr{\mright}

\makeatletter
\newcommand{\tdb}[1]{\colorbox{lime}{$\displaystyle #1$}}
\newcommand{\defeq}{:=}
\newcommand{\uset}[1]{\{#1\}}
\newcommand{\otup}[1]{\langle#1\rangle}
\newcommand{\enlist}[2]{{#1}_{1}, {#1}_{2}, {#1}_{3}, \cdots, {#1}_{#2}}
\newcommand{\cusand}{,}
\newcommand{\cuspop}{.}
\newcommand{\eqComment}[1]{\text{  \# #1}}
\newcommand{\eqSep}{\text{ ;  }}
\newcommand{\n}{\\[1.5ex] \hline \nonumber \\[0ex]}
\newcommand{\m}{\nonumber \\}
\newcommand{\sfield}[1]{\textbf{\textit{#1}}}

%%%%%%%%%%%%%%%%%%
\newcommand{\dfnNEW}[2]{\textcolor{teal}{%
  \hypertarget{#1}{#2}%
    \protected@write\@mainaux{}{%
        \string\expandafter\string\gdef
          \string\csname\string\detokenize{#1}\string\endcsname{#2}%
    }%
  }}
\DeclareDocumentCommand{\dfn}{m o}{%
  \dfnNEW{#1}{\IfNoValueTF{#2}{#1}{#2}}
  }
  
\newcommand{\rfrNEW}[1]{%
  \hyperlink{#1}{\csname #1\endcsname}%
  }
%\newcommand{\rfr}[1]{% maybe optional this as well
%  \ifcsname#1\endcsname%
%    \rfrNEW{#1}%
%  \else%
%    \textcolor{red}{#1^!}% undefined
%  \fi%
%}
\DeclareDocumentCommand{\rfr}{m o o}{%
  \ifcsname#1\endcsname%
    \IfNoValueTF{#3}{\IfNoValueTF{#2}{
      \rfrNEW{#1}}{
      \rfrNEW{#1} #2}}{
      (#2 \rfrNEW{#1} #3)}
  \else%
    \textcolor{red}{\space^!#1}% undefined
  \fi%
}

%%%%%%%%%%%%%%%%%%
\newcommand\rfrlist[1]{%
    \forcsvlist{\rfrlist@item}{#1}
}
\newcommand\rfrlist@item[1]{\rfr{#1}\\}
\newcommand{\thmlink}[2]{{}_{\substack{\rfrlist{#1}}}^{\dfn{#2}} }
\makeatother

\title{Next-Next-Gen Notes \\
\large Object-Oriented Maths}
\author{JP Guzman}

\begin{document}
\maketitle
\allowdisplaybreaks


\thinmuskip=2mu % commas
\medmuskip=2mu % operators
\thickmuskip=2mu % equalities
\setlength{\belowdisplayskip}{0pt} \setlength{\belowdisplayshortskip}{0pt}
\setlength{\abovedisplayskip}{0pt} \setlength{\abovedisplayshortskip}{0pt}

% https://en.wikipedia.org/wiki/List_of_mathematical_abbreviations

\section{Mathematical Logic}
\subsection{NaiveMaster}
\tdb{\textbf{undefined terms}:} $%
   \dfn{set}, %
   \dfn{tuple}, %
   \dfn{element}, % 
   \dfn{nnumber}, %
   \dfn{-in}[\in], %
   \dfn{-subset}[\subseteq], %
   \dfn{-eq}[=], %
   \dfn{-not}[\not] \ , %
   \dfn{-psubset}[\subset], %
   \dfn{-union}[\cup], %
   \dfn{-intersection}[\cap], %
   \dfn{empty-set}[\emptyset], %
   \dfn{usetl}[\{], %
   \dfn{usetr}[\}], %
   \dfn{otupl}[\langle], %
   \dfn{otupr}[\rangle], %
   \dfn{st}[\mid], %
   \dfn{ktupset}[\widehat{\ }], %
   \dfn{cartesian}[\times], %
   \dfn{relation}, %
   \dfn{property}, %
   \dfn{binaryRelation}, %
     \\ %
   \dfn{domain}, %
   \dfn{range}, %
   \dfn{field}, %
$
\begin{tcolorbox}[breakable, enhanced]
\begin{align}
\n \rfr{element} [x][] \rfr{-in} \rfr{set} [y][] %
%%%\rfr{-in}[\rfr{element} [x][]][\rfr{set} [y][]]
\m \eqComment{x belongs to y}
\n \rfr{set} [x][] \rfr{-subset} \rfr{set} [y][]
\m \eqComment{x is included in y}
\n \rfr{set} [x][] \rfr{-eq} \rfr{set} [y][] \defeq (\rfr{set} [x][] \rfr{-subset} \rfr{set} [y][], \rfr{set} [y][] \rfr{-subset} \rfr{set} [x][])
\m \eqComment{x is the same set as y}
\n \rfr{set} [x][] \rfr{-psubset} \rfr{set} [y][] ((= x \nsubseteq y)) \defeq \rfr{set} [x][] \subseteq \rfr{set} [y][], \rfr{set} [x][] \rfr{-not} \rfr{-eq} \rfr{set} [y][]
\m \eqComment{x is a proper subset of y}
\n \rfr{set} [x][] \rfr{-union} \rfr{set} [y][]
\m \eqComment{all elements in x or y}
\n \rfr{set} [x][] \rfr{-intersection} \rfr{set} [y][]
\m \eqComment{all elements in x and y}
\n \dfn{disjoint} [x, y][] \defeq \rfr{set} [x][] \rfr{-intersection} \rfr{set} [y][] \rfr{-eq} \rfr{empty-set}
\m \eqComment{disjoint sets do not intersect}
\n \rfr{set} [E][] \rfr{-eq} \rfr{usetl} \enlist{e}{n} \rfr{usetr}
\m \eqComment{unordered set containing $\enlist{e}{n}$}
\m \rfr{usetl} e_1, e_2, e_3 \rfr{usetr} \rfr{-eq} \rfr{usetl} e_3, e_1, e_2 \rfr{usetr}
\n \rfr{tuple} [E][] \rfr{-eq} \rfr{otupl} \enlist{e}{n} \rfr{otupr} 
\m \eqComment{ordered tuple containing $\enlist{e}{n}$}
\m \rfr{otupl} e_1, e_2, e_3 \rfr{otupr} \rfr{-not} \rfr{-eq} \rfr{otupl} e_2, e_3, e_1 \rfr{otupr}
\n \rfr{set} [X][] \rfr{ktupset} \rfr{nnumber} [k][]
\m \eqComment{set of all ordered k-tuples from the elements in X}
\m X \rfr{ktupset} 1 \rfr{-eq} \rfr{usetl} \enlist{e}{n} \rfr{usetr} \rfr{ktupset} 1 \rfr{-eq} \rfr{usetl} \rfr{otupl} e_1 \rfr{otupr}, \rfr{otupl} e_2 \rfr{otupr}, \rfr{otupl} e_3 \rfr{otupr}, \cdots, \rfr{otupl} e_n \rfr{otupr} \rfr{usetr} = \rfr{usetl} \enlist{e}{n} \rfr{usetr} \rfr{-eq} X
\n \rfr{set} [Y][] \rfr{times} \rfr{set} [Z][]
\m \eqComment{Cartesian product}
\n \rfr{relation} [R][S, k] \rfr{-subset} \rfr{set} [S][] \rfr{ktupset} \rfr{nnumber} [k][]
\m \eqComment{k-tuple relation R on the set S takes only tuples that satisfy some relation}
\n \rfr{property} [P][S] \rfr{-eq} \rfr{relation} [P][S, 1] \rfr{-subset} \rfr{set} [S][] \rfr{ktupset} 1 \rfr{-eq} S
\m \eqComment{property P of the set S}
\n \rfr{binaryRelation} [B][S] \rfr{-eq} \rfr{relation} [B][S, 2] \rfr{-subset} \rfr{set} [S][] \rfr{ktupset} 2
\m x B y \rfr{-eq} \rfr{otupl} x, y \rfr{otupr} \rfr{-in} B 
\n \rfr{domain} [X][B, S] \rfr{-eq} \rfr{usetl} x \rfr{st} \rfr{otupl} x, y \rfr{otupr} \rfr{-in} \rfr{binaryRelation} [B][S] \rfr{usetr}
\n \rfr{range} [Y][B, S] \rfr{-eq} \rfr{usetl} y \rfr{st} \rfr{otupl} x, y \rfr{otupr} \rfr{-in} \rfr{binaryRelation} [B][S] \rfr{usetr}
\n \rfr{field} [F][B, S] \rfr{-eq} \rfr{domain} [X][B, S] \rfr{-union} \rfr{range} [Y][B, S]
\n \dfn{inverseRelation} [B^{-1}][B, S] \defeq \rfr{usetl} \rfr{otupl} y, x \rfr{otupr} \rfr{st} \rfr{otupl} x, y \rfr{otupr} \rfr{-in} \rfr{binaryRelation} [B][S] \rfr{usetr}
\n \dfn{reflexive} [B][S] \defeq x \rfr{-in} \rfr{field} [F][B, S], x B x define forall not in set, quantifiers, if and or etc.
\n \dfn{symmetric} [B][S] \defeq
\n \dfn{transitive} [B][S] \defeq
\n000000000000000000000000000000000000000000000000000000000000000000000000000000000000000  
\m \otup{a, b} \in inverse(R^{-1}) : \otup{b, a} \in R 
\m reflexive(R^2_X) : x R^2_X x
\m symmetric(R^2_X) : x R^2_X y = y R^2_X x
\m transitive(R^2_X) : x R^2_X y, y R^2_X z : x R^2_X z
\m equivalenceRelation(R^2_X) := reflexive(R^2_X), symmetric(R^2_X), transitive(R^2_X)
\n take this intro shit more srsly 
\end{align}
\end{tcolorbox}

\section{Logic and Set Theory}
\subsection{Logical Truths and Operators}
\begin{tcolorbox}[breakable, enhanced]
\begin{align}
\n \dfn{truth} [t][] \defeq t = \begin{cases} \dfn{T} \\ \dfn{F} \end{cases} 
\n \dfn{statement} [s][] \defeq \rfr{correctSyntaxSemantics} [s][] 
\n \dfn{proposition} [s, t][] \defeq \ml(\rfr{statement} [s][]\mr) \cusand \ml(\rfr{truth} [t][]\mr) \cuspop
\n \dfn{operatorOR} [\dfn{OR}[\lor]][x, y] \defeq \ml(\rfr{truth} [x][]\mr) \cusand \ml(\rfr{truth} [y][]\mr) \cusand \ml(\rfr{truth} [x \rfr{OR} y][] = \begin{cases} \rfr{F} & x = \rfr{F} \cusand y = \rfr{F} \\ \rfr{T} & x = \rfr{F} \cusand y = \rfr{T} \\ \rfr{T} & x = \rfr{T} \cusand y = \rfr{F} \\ \rfr{T} & x = \rfr{T} \cusand y = \rfr{T} \end{cases}\mr) \cuspop
\n \dfn{operatorAND} [\dfn{AND}[\land]][x, y] \defeq \ml(\rfr{truth} [x][]\mr) \cusand \ml(\rfr{truth} [y][]\mr) \cusand \ml(\rfr{truth} [x \rfr{AND} y][] = \begin{cases} \rfr{F} & x = \rfr{F} \cusand y = \rfr{F} \\ \rfr{F} & x = \rfr{F} \cusand y = \rfr{T} \\ \rfr{F} & x = \rfr{T} \cusand y = \rfr{F} \\ \rfr{T} & x = \rfr{T} \cusand y = \rfr{T} \end{cases}\mr) \cuspop
\n \dfn{operatorNOT} [\dfn{NOT}[\lnot]][x] \defeq \ml(\rfr{truth} [x][]\mr) \cusand \ml(\rfr{truth} [\rfr{NOT} x][] = \begin{cases} \rfr{T} & x = \rfr{F} \\ \rfr{F} & x = \rfr{T} \end{cases}\mr) \cuspop 
\n \dfn{booleanAlgebra} [\{\rfr{T}, \rfr{F}\}, \rfr{AND}, \rfr{OR}, \rfr{NOT}][] \defeq \thmlink{}{POS-LCom} \ml(\ml(x \rfr{AND} y = y \rfr{AND} x\mr) \cusand \ml(x \rfr{OR} y = y \rfr{OR} x\mr)\mr) \eqComment{Commutative} \cusand
\m \thmlink{}{POS-LDis} \ml(\ml(x \rfr{AND} \ml(y \rfr{OR} z\mr) = \ml(x \rfr{AND} y\mr) \rfr{OR} \ml(x \rfr{AND} z\mr)\mr) \cusand \ml(x \rfr{OR} \ml(y \rfr{AND} z\mr) = \ml(x \rfr{OR} y\mr) \rfr{AND} \ml(x \rfr{OR} z\mr)\mr)\mr) \eqComment{Distributive} \cusand
\m \thmlink{}{POS-LIdn} \ml(\ml(x \rfr{AND} \rfr{T} = x\mr) \cusand \ml(x \rfr{OR} \rfr{F} = x\mr)\mr) \eqComment{Identity} \cusand
\m \thmlink{}{POS-LCmp} \ml(\ml(x \rfr{AND} \rfr{NOT} x = \rfr{F}\mr) \cusand \ml(x \rfr{OR} \rfr{NOT} x = \rfr{T}\mr)\mr) \eqComment{Complement} \cuspop
\n \dfn{operatorXOR} [\dfn{XOR}[\veebar]][x, y] \defeq \ml(\rfr{truth} [x][]\mr) \cusand \ml(\rfr{truth} [y][]\mr) \cusand \ml(\rfr{truth} [x \rfr{XOR} y][] = \begin{cases} \rfr{F} & x = \rfr{F} \cusand y = \rfr{F} \\ \rfr{T} & x = \rfr{F} \cusand y = \rfr{T} \\ \rfr{T} & x = \rfr{T} \cusand y = \rfr{F} \\ \rfr{F} & x = \rfr{T} \cusand y = \rfr{T} \end{cases}\mr) \cuspop
\n \dfn{operatorIF} [\dfn{IF}[\implies]][x, y] \defeq \ml(\rfr{truth} [x][]\mr) \cusand \ml(\rfr{truth} [y][]\mr) \cusand \ml(\rfr{truth} [x \rfr{IF} y][] = \ml(\rfr{NOT} x\mr) \rfr{OR} y = \begin{cases} \rfr{T} & x = \rfr{F} \cusand y = \rfr{F} \\ \rfr{T} & x = \rfr{F} \cusand y = \rfr{T} \\ \rfr{F} & x = \rfr{T} \cusand y = \rfr{F} \\ \rfr{T} & x = \rfr{T} \cusand y = \rfr{T} \end{cases}\mr) \cuspop
\n \thmlink{POS-LCmp}{THM-LExp-1} \ml(\rfr{F} = x \rfr{AND} \rfr{NOT} x\mr) \rfr{IF}
\m \thmlink{THM-LExp-1}{THM-LExp-2} \ml(x\mr) \cusand
\m \thmlink{THM-LExp-1}{THM-LExp-3} \ml(\rfr{NOT} x\mr) \cusand
\m \thmlink{THM-LExp-2}{THM-LExp-4} \ml(x \rfr{OR} y\mr) \cusand
\m \thmlink{THM-LExp-4, THM-LExp-3}{THM-LExp-5} \ml(y\mr) \cuspop
\m \thmlink{THM-LExp-1, THM-LExp-2, THM-LExp-3, THM-LExp-4, THM-LExp-5}{THM-LExp} \ml(\rfr{F} \rfr{IF} y\mr)
\m \eqComment{The Principle of Explosion, anything follows from a false $\ml(\rfr{F}\mr)$ premise}
\n \dfn{operatorOIF} [\dfn{OIF}[\impliedby]][x, y] \defeq \ml(\rfr{truth} [x][]\mr) \cusand \ml(\rfr{truth} [y][]\mr) \cusand \ml(\rfr{truth} [x \rfr{OIF} y][] = \ml(\rfr{NOT} y\mr) \rfr{OR} x = \begin{cases} \rfr{T} & x = \rfr{F} \cusand y = \rfr{F} \\ \rfr{F} & x = \rfr{F} \cusand y = \rfr{T} \\ \rfr{T} & x = \rfr{T} \cusand y = \rfr{F} \\ \rfr{T} & x = \rfr{T} \cusand y = \rfr{T} \end{cases}\mr) \cuspop
\n \dfn{operatorIIF} [\dfn{IFF}[\iff]][x, y] \defeq \ml(\rfr{truth} [x][]\mr) \cusand \ml(\rfr{truth} [y][]\mr) \cusand 
\m \ml(\rfr{truth} [x \rfr{IFF} y][] = (x \rfr{IF} y) \rfr{AND} (y \rfr{IF} x) = \begin{cases} \rfr{T} & x = \rfr{F} \cusand y = \rfr{F} \\ \rfr{F} & x = \rfr{F} \cusand y = \rfr{T} \\ \rfr{F} & x = \rfr{T} \cusand y = \rfr{F} \\ \rfr{T} & x = \rfr{T} \cusand y = \rfr{T} \end{cases}\mr) \cuspop
\end{align}
\end{tcolorbox}

\begin{comment}

\subsection{Boolean Algebra Properties}
\begin{tcolorbox}[breakable, enhanced]
\begin{align}
   \thmlink{POS-LCom}{THM-Dual-1} \Bigg(\rfrOLD{booleanAlgebra}[\{\rfrOLD{T}, \rfrOLD{F}\}, \rfrOLD{\land}, \rfrOLD{\lor}, \rfrOLD{\lnot}][] \rfrOLD{\iff}
\m \ml(\ml(x \rfrOLD{\lor} y = y \rfrOLD{\lor} x\mr) \cusand \ml(x \rfrOLD{\land} y = y \rfrOLD{\land} x\mr)\mr) \eqComment{Reordered Commutative} \cusand
\m \ml(\ml(x \rfrOLD{\lor} \ml(y \rfrOLD{\land} z\mr) = \ml(x \rfrOLD{\lor} y\mr) \rfrOLD{\land} \ml(x \rfrOLD{\lor} z\mr)\mr) \cusand \ml(x \rfrOLD{\land} \ml(y \rfrOLD{\lor} z\mr) = \ml(x \rfrOLD{\land} y\mr) \rfrOLD{\lor} \ml(x \rfrOLD{\land} z\mr)\mr)\mr) \eqComment{Reordered Distributive} \cusand
\m \ml(\ml(x \rfrOLD{\lor} \rfrOLD{F} = x\mr) \cusand \ml(x \rfrOLD{\land} \rfrOLD{T} = x\mr)\mr) \eqComment{Reordered Identity} \cusand
\m \ml(\ml(x \rfrOLD{\lor} \rfrOLD{\lnot} x = \rfrOLD{T}\mr) \cusand \ml(x \rfrOLD{\land} \rfrOLD{\lnot} x = \rfrOLD{F}\mr)\mr) \eqComment{Reordered Complement} \cuspop \rfrOLD{\iff}
\m \rfrOLD{booleanAlgebra}[\{\rfrOLD{F}, \rfrOLD{T}\}, \rfrOLD{\lor}, \rfrOLD{\land}, \rfrOLD{\lnot}][]\Bigg)
\m \thmlink{THM-Dual-1}{THM-Dual} \ml(\rfrOLD{booleanAlgebra}[\{\rfrOLD{T}, \rfrOLD{F}\}, \rfrOLD{\land}, \rfrOLD{\lor}, \rfrOLD{\lnot}][] \rfrOLD{\iff} \rfrOLD{booleanAlgebra}[\{\rfrOLD{F}, \rfrOLD{T}\}, \rfrOLD{\lor}, \rfrOLD{\land}, \rfrOLD{\lnot}][]\mr)
\m \eqComment{Boolean Algebra Duality follows from the swap symmetry of $\ml(\rfrOLD{\land}, \rfrOLD{T}\mr)$ and $\ml(\rfrOLD{\lor}, \rfrOLD{F}\mr)$ within the axioms}
\n \thmlink{}{THM-LUNt-1} \ml(\ml(x \rfrOLD{\lor} y = \rfrOLD{T} = x \rfrOLD{\lor} z\mr) \rfrOLD{\land} \ml(x \rfrOLD{\land} y = \rfrOLD{F} = x \rfrOLD{\land} z\mr)\mr) \rfrOLD{\implies}
\m \thmlink{POS-LIdn}{THM-LUNt-2} \ml(y = y \rfrOLD{\land} \rfrOLD{T}\mr) \cusand
\m \thmlink{THM-LUNt-1}{THM-LUNt-3} \ml(y \rfrOLD{\land} \rfrOLD{T} = y \rfrOLD{\land} \ml(x \rfrOLD{\lor} z\mr)\mr) \cusand
\m \thmlink{POS-LDis}{THM-LUNt-4} \ml(y \rfrOLD{\land} \ml(x \rfrOLD{\lor} z\mr) = \ml(y \rfrOLD{\land} x\mr) \rfrOLD{\lor} \ml(y \rfrOLD{\land} z\mr)\mr) \cusand
\m \thmlink{POS-LCom, THM-LUNt-4}{THM-LUNt-5} \ml(\ml(y \rfrOLD{\land} x\mr) \rfrOLD{\lor} \ml(y \rfrOLD{\land} z\mr) = \ml(x \rfrOLD{\land} z\mr) \rfrOLD{\lor} \ml(y \rfrOLD{\land} z\mr)\mr) \cusand
\m \thmlink{POS-LCom, POS-LDis}{THM-LUNt-6} \ml(\ml(x \rfrOLD{\land} z\mr) \rfrOLD{\lor} \ml(y \rfrOLD{\land} z\mr) = z \rfrOLD{\land} \ml(x \rfrOLD{\lor} y\mr)\mr) \cusand
\m \thmlink{THM-LUNt-1}{THM-LUNt-7} \ml(z \rfrOLD{\land} \ml(x \rfrOLD{\lor} y\mr) = z \rfrOLD{\land} \rfrOLD{T}\mr) \cusand
\m \thmlink{POS-LIdn}{THM-LUNt-8} \ml(z \rfrOLD{\land} \rfrOLD{T} = z\mr) \cuspop
\m \thmlink{THM-LUNt-1, THM-LUNt-2, THM-LUNt-3, THM-LUNt-4, THM-LUNt-5, THM-LUNt-6, THM-LUNt-7, THM-LUNt-8}{THM-LUNt} \ml(\ml(\ml(x \rfrOLD{\lor} y = \rfrOLD{T} = x \rfrOLD{\lor} z\mr) \rfrOLD{\land} \ml(x \rfrOLD{\land} y = \rfrOLD{F} = x \rfrOLD{\land} z\mr)\mr) \rfrOLD{\implies} \ml(y = z\mr)\mr)
\m \eqComment{Uniqueness of Complements}
\n \thmlink{POS-LIdn}{THM-LDom-1} \ml(x \rfrOLD{\lor} \rfrOLD{T} = \ml(x \rfrOLD{\lor} \rfrOLD{T}\mr) \rfrOLD{\land} \rfrOLD{T}\mr) \cusand
\m \thmlink{POS-LCmp}{THM-LDom-2} \ml(\ml(x \rfrOLD{\lor} \rfrOLD{T}\mr) \rfrOLD{\land} \rfrOLD{T} = \ml(x \rfrOLD{\lor} \rfrOLD{T}\mr) \rfrOLD{\land} \ml(x \rfrOLD{\lor} \rfrOLD{\lnot} x\mr)\mr) \cusand
\m \thmlink{POS-LDis}{THM-LDom-3} \ml(\ml(x \rfrOLD{\lor} \rfrOLD{T}\mr) \rfrOLD{\land} \ml(x \rfrOLD{\lor} \rfrOLD{\lnot} x\mr) = x \rfrOLD{\lor} \ml(\rfrOLD{T} \rfrOLD{\land} \rfrOLD{\lnot} x\mr)\mr) \cusand
\m \thmlink{POS-LIdn}{THM-LDom-4} \ml(x \rfrOLD{\lor} \ml(\rfrOLD{T} \rfrOLD{\land} \rfrOLD{\lnot} x\mr) = x \rfrOLD{\lor} \rfrOLD{\lnot} x\mr) \cusand
\m \thmlink{POS-LCmp}{THM-LDom-5} \ml(x \rfrOLD{\lor} \rfrOLD{\lnot} x = \rfrOLD{T}\mr) \cuspop
\m \thmlink{THM-LDom-1, THM-LDom-2, THM-LDom-3, THM-LDom-4, THM-LDom-5}{THM-LDom-6} \ml(x \rfrOLD{\lor} \rfrOLD{T} = \rfrOLD{T}\mr) \cusand
\m \thmlink{THM-LDom-6, THM-Dual}{THM-LDom} \ml(\ml(x \rfrOLD{\lor} \rfrOLD{T} = \rfrOLD{T}\mr) \cusand \ml(x \rfrOLD{\land} \rfrOLD{F} = \rfrOLD{F}\mr)\mr) \cuspop
\m \eqComment{Domination}
\n \thmlink{POS-LIdn}{THM-LIdm-1} \ml(x \rfrOLD{\lor} x = \ml(x \rfrOLD{\lor} x\mr) \rfrOLD{\land} \rfrOLD{T}\mr) \cusand
\m \thmlink{POS-LCmp}{THM-LIdm-2} \ml(\ml(x \rfrOLD{\lor} x\mr) \rfrOLD{\land} \rfrOLD{T} = \ml(x \rfrOLD{\lor} x\mr) \rfrOLD{\land} \ml(x \rfrOLD{\lor} \rfrOLD{\lnot} x\mr)\mr) \cusand
\m \thmlink{POS-LDis}{THM-LIdm-3} \ml(\ml(x \rfrOLD{\lor} x\mr) \rfrOLD{\land} \ml(x \rfrOLD{\lor} \rfrOLD{\lnot} x\mr) = x \rfrOLD{\land} \ml(x \rfrOLD{\lor} \rfrOLD{\lnot} x\mr)\mr) \cusand
\m \thmlink{POS-LCmp}{THM-LIdm-4} \ml(x \rfrOLD{\land} \ml(x \rfrOLD{\lor} \rfrOLD{\lnot} x\mr) = x \rfrOLD{\land} \rfrOLD{T}\mr) \cusand
\m \thmlink{POS-LIdn}{THM-LIdm-5} \ml(x \rfrOLD{\land} \rfrOLD{T} = x\mr) \cusand
\m \thmlink{THM-LIdm-1, THM-LIdm-2, THM-LIdm-3, THM-LIdm-4, THM-LIdm-5}{THM-LIdm-6} \ml(x \rfrOLD{\lor} x = x\mr) \cusand
\m \thmlink{THM-LIdm-6, THM-Dual}{THM-LIdm} \ml(\ml(x \rfrOLD{\lor} x = x\mr) , \ml(x \rfrOLD{\land} x = x\mr)\mr) \cuspop
\m \eqComment{Idempotent}
\n \thmlink{POS-LIdn}{THM-LInv-1} \ml(\rfrOLD{\lnot} \rfrOLD{\lnot} x = \rfrOLD{\lnot} \rfrOLD{\lnot} x \rfrOLD{\lor} \rfrOLD{F}\mr) \cusand
\m \thmlink{POS-LCmp}{THM-LInv-2} \ml(\rfrOLD{\lnot} \rfrOLD{\lnot} x \rfrOLD{\lor} \rfrOLD{F} = \rfrOLD{\lnot} \rfrOLD{\lnot} x \rfrOLD{\lor} \ml(x \rfrOLD{\land} \rfrOLD{\lnot} x\mr)\mr) \cusand
\m \thmlink{POS-LDis}{THM-LInv-3} \ml(\rfrOLD{\lnot} \rfrOLD{\lnot} x \rfrOLD{\lor} \ml(x \rfrOLD{\land} \rfrOLD{\lnot} x\mr)= \ml(\rfrOLD{\lnot} \rfrOLD{\lnot} x \rfrOLD{\lor} x\mr) \rfrOLD{\land} \ml(\rfrOLD{\lnot} \rfrOLD{\lnot} x \rfrOLD{\lor} \rfrOLD{\lnot} x\mr)\mr) \cusand
\m \thmlink{POS-LCmp}{THM-LInv-4} \ml(\ml(\rfrOLD{\lnot} \rfrOLD{\lnot} x \rfrOLD{\lor} x\mr) \rfrOLD{\land} \ml(\rfrOLD{\lnot} \rfrOLD{\lnot} x \rfrOLD{\lor} \rfrOLD{\lnot} x\mr) = \ml(\rfrOLD{\lnot} \rfrOLD{\lnot} x \rfrOLD{\lor} x\mr) \rfrOLD{\land} \rfrOLD{T}\mr) \cusand
\m \thmlink{POS-LCmp}{THM-LInv-5} \ml(\ml(\rfrOLD{\lnot} \rfrOLD{\lnot} x \rfrOLD{\lor} x\mr) \rfrOLD{\land} \rfrOLD{T} = \ml(\rfrOLD{\lnot} \rfrOLD{\lnot} x \rfrOLD{\lor} x\mr) \rfrOLD{\land} \ml(x \rfrOLD{\lor} \rfrOLD{\lnot} x\mr)\mr) \cusand
\m \thmlink{POS-LDis}{THM-LInv-6} \ml(\ml(\rfrOLD{\lnot} \rfrOLD{\lnot} x \rfrOLD{\lor} x\mr) \rfrOLD{\land} \ml(x \rfrOLD{\lor} \rfrOLD{\lnot} x\mr) = x \rfrOLD{\lor} \ml(\rfrOLD{\lnot} \rfrOLD{\lnot} x \rfrOLD{\land} \rfrOLD{\lnot} x\mr)\mr) \cusand
\m \thmlink{POS-LCmp}{THM-LInv-7} \ml(x \rfrOLD{\lor} \ml(\rfrOLD{\lnot} \rfrOLD{\lnot} x \rfrOLD{\land} \rfrOLD{\lnot} x\mr)= x \rfrOLD{\lor} \rfrOLD{F}\mr) \cusand
\m \thmlink{POS-LIdn}{THM-LInv-8} \ml(x \rfrOLD{\lor} \rfrOLD{F} = x\mr) \cusand
\m \thmlink{THM-LInv-1, THM-LInv-2, THM-LInv-3, THM-LInv-4, THM-LInv-5, THM-LInv-6, THM-LInv-7, THM-LInv-8}{THM-LInv} \ml(\rfrOLD{\lnot} \rfrOLD{\lnot} x = x\mr) \cuspop
\m \eqComment{Involution}
\n \thmlink{POS-LIdn}{THM-LAbs-1} \ml(x \rfrOLD{\lor} \ml(x \rfrOLD{\land} y\mr) = \ml(x \rfrOLD{\land} \rfrOLD{T}\mr) \rfrOLD{\lor} \ml(x \rfrOLD{\land} y\mr)\mr) \cusand
\m \thmlink{POS-LDis}{THM-LAbs-2} \ml(\ml(x \rfrOLD{\land} \rfrOLD{T}\mr) \rfrOLD{\lor} \ml(x \rfrOLD{\land} y\mr) = x \rfrOLD{\land} \ml(\rfrOLD{T} \rfrOLD{\lor} y\mr)\mr) \cusand
\m \thmlink{THM-LDom}{THM-LAbs-3} \ml(x \rfrOLD{\land} \ml(\rfrOLD{T} \rfrOLD{\lor} y\mr) = x \rfrOLD{\land} \rfrOLD{T}\mr) \cusand
\m \thmlink{THM-LIdn}{THM-LAbs-4} \ml(x \rfrOLD{\land} \rfrOLD{T} = x\mr) \cusand
\m \thmlink{THM-LAbs-1, THM-LAbs-2, THM-LAbs-3, THM-LAbs-4}{THM-LAbs-5} \ml(x \rfrOLD{\lor} \ml(x \rfrOLD{\land} y\mr) = x\mr) \cusand
\m \thmlink{THM-LAbs-5, THM-Dual}{THM-LAbs} \ml(\ml(x \rfrOLD{\lor} \ml(x \rfrOLD{\land} y\mr) = x\mr) \cusand \ml(x \rfrOLD{\land} \ml(x \rfrOLD{\lor} y\mr) = x\mr)\mr) \cuspop
\m \eqComment{Absorption}
\n \thmlink{}{THM-LAsc-1} ((A = x \rfrOLD{\lor} (y \rfrOLD{\lor} z)) \cusand (B = (x \rfrOLD{\lor} y) \rfrOLD{\lor} z)) \rfrOLD{\implies}
\m \thmlink{THM-LAsc-1}{THM-LAsc-2} (x \rfrOLD{\land} A = x \rfrOLD{\land} (x \rfrOLD{\lor} (y \rfrOLD{\lor} z))) \cusand \cusand
\m \thmlink{THM-LAbs}{THM-LAsc-3} (x \rfrOLD{\land} (x \rfrOLD{\lor} (y \rfrOLD{\lor} z)) = x) \cusand \cusand
\m \thmlink{THM-LAsc-1}{THM-LAsc-4} (x \rfrOLD{\land} B = x \rfrOLD{\land} ((x \rfrOLD{\lor} y) \rfrOLD{\lor} z)) \cusand \cusand
\m \thmlink{POS-LDis}{THM-LAsc-5} (x \rfrOLD{\land} ((x \rfrOLD{\lor} y) \rfrOLD{\lor} z) = (x \rfrOLD{\land} (x \rfrOLD{\lor} y)) \rfrOLD{\lor} (x \rfrOLD{\land} z)) \cusand \cusand
\m \thmlink{THM-LAbs}{THM-LAsc-6} ((x \rfrOLD{\land} (x \rfrOLD{\lor} y)) \rfrOLD{\lor} (x \rfrOLD{\land} z) = x \rfrOLD{\lor} (x \rfrOLD{\land} z)) \cusand \cusand
\m \thmlink{THM-LAbs}{THM-LAsc-7} (x \rfrOLD{\lor} (x \rfrOLD{\land} z) = x) \cusand \cusand
\m \thmlink{THM-LAbs}{THM-LAsc-8} ((x \rfrOLD{\land} (x \rfrOLD{\lor} y)) \rfrOLD{\lor} (x \rfrOLD{\land} z) = x \rfrOLD{\lor} (x \rfrOLD{\land} z)) \cusand \cusand
\m \thmlink{THM-LAsc-2, THM-LAsc-3, THM-LAsc-4, THM-LAsc-5, THM-LAsc-6, THM-LAsc-7, THM-LAsc-8}{THM-LAsc-9} (x \rfrOLD{\land} A = x = x \rfrOLD{\land} B) \cuspop \cusand
\m \thmlink{THM-LAsc-1}{THM-LAsc-10} (\rfrOLD{\lnot} x \rfrOLD{\land} A = \rfrOLD{\lnot} x \rfrOLD{\land} (x \rfrOLD{\lor} (y \rfrOLD{\lor} z))) \cusand \cusand
\m \thmlink{POS-LDis}{THM-LAsc-11} (\rfrOLD{\lnot} x \rfrOLD{\land} (x \rfrOLD{\lor} (y \rfrOLD{\lor} z)) = (\rfrOLD{\lnot} x \rfrOLD{\land} x) \rfrOLD{\lor} (\rfrOLD{\lnot} x \rfrOLD{\land} (y + z))) \cusand \cusand
\m \thmlink{POS-LCmp}{THM-LAsc-12} ((\rfrOLD{\lnot} x \rfrOLD{\land} x) \rfrOLD{\lor} (\rfrOLD{\lnot} x \rfrOLD{\land} (y \rfrOLD{\lor} z)) = \rfrOLD{F} \rfrOLD{\lor} (\rfrOLD{\lnot} x \rfrOLD{\land} (y \rfrOLD{\lor} z))) \cusand \cusand
\m \thmlink{POS-LIdn}{THM-LAsc-13} (\rfrOLD{F} \rfrOLD{\lor} (\rfrOLD{\lnot} x \rfrOLD{\land} (y + z)) = \rfrOLD{\lnot} x \rfrOLD{\land} (y \rfrOLD{\lor} z)) \cusand \cusand
\m \thmlink{THM-LAsc-1}{THM-LAsc-14} (\rfrOLD{\lnot} x \rfrOLD{\land} B = \rfrOLD{\lnot} x \rfrOLD{\land} ((x \rfrOLD{\lor} y) \rfrOLD{\lor} z)) \cusand \cusand
\m \thmlink{POS-LDis}{THM-LAsc-15} (\rfrOLD{\lnot} x \rfrOLD{\land} ((x \rfrOLD{\lor} y) \rfrOLD{\lor} z) = (\rfrOLD{\lnot} x \rfrOLD{\land} (x \rfrOLD{\lor} y)) \rfrOLD{\lor} (\rfrOLD{\lnot} x \rfrOLD{\land} z)) \cusand \cusand
\m \thmlink{POS-LDis}{THM-LAsc-16} ((\rfrOLD{\lnot} x \rfrOLD{\land} (x \rfrOLD{\lor} y)) \rfrOLD{\lor} (\rfrOLD{\lnot} x \rfrOLD{\land} z) = ((\rfrOLD{\lnot} x \rfrOLD{\land} x) \rfrOLD{\lor} (\rfrOLD{\lnot} x \rfrOLD{\land} y)) \rfrOLD{\lor} (\rfrOLD{\lnot} x \rfrOLD{\land} z)) \cusand \cusand
\m \thmlink{POS-LCmp}{THM-LAsc-17} (((\rfrOLD{\lnot} x \rfrOLD{\land} x) \rfrOLD{\lor} (\rfrOLD{\lnot} x \rfrOLD{\land} y)) \rfrOLD{\lor} (\rfrOLD{\lnot} x \rfrOLD{\land} z) = (\rfrOLD{F} \rfrOLD{\lor} (\rfrOLD{\lnot} x \rfrOLD{\land} y)) \rfrOLD{\lor} (\rfrOLD{\lnot} x \rfrOLD{\land} z)) \cusand \cusand
\m \thmlink{POS-LIdn}{THM-LAsc-18} ((\rfrOLD{F} \rfrOLD{\lor} (\rfrOLD{\lnot} x \rfrOLD{\land} y)) \rfrOLD{\lor} (\rfrOLD{\lnot} x \rfrOLD{\land} z) = (\rfrOLD{\lnot} x \rfrOLD{\land} y) \rfrOLD{\lor} (\rfrOLD{\lnot} x \rfrOLD{\land} z)) \cusand \cusand
\m \thmlink{POS-LDis}{THM-LAsc-19} ((\rfrOLD{\lnot} x \rfrOLD{\land} y) \rfrOLD{\lor} (\rfrOLD{\lnot} x \rfrOLD{\land} z) = \rfrOLD{\lnot} x \rfrOLD{\land} (y \rfrOLD{\lor} z)) \cusand \cusand
\m \thmlink{THM-LAsc-10, THM-LAsc-11, THM-LAsc-12, THM-LAsc-13, THM-LAsc-14, THM-LAsc-15, THM-LAsc-16, THM-LAsc-17, THM-LAsc-18, THM-LAsc-19}{THM-LAsc-20} (\rfrOLD{\lnot} x \rfrOLD{\land} A = \rfrOLD{\lnot} x \rfrOLD{\land} (y \rfrOLD{\lor} z) = \rfrOLD{\lnot} x \rfrOLD{\land} B) \cuspop \cusand
\m \thmlink{POS-LDis}{THM-LAsc-21} (A = A \rfrOLD{\land} \rfrOLD{T}) \cusand \cusand
\m \thmlink{POS-LCmp}{THM-LAsc-22} (A \rfrOLD{\land} \rfrOLD{T} = A \rfrOLD{\land} (x \rfrOLD{\lor} \rfrOLD{\lnot} x)) \cusand \cusand
\m \thmlink{POS-LDis}{THM-LAsc-23} (A \rfrOLD{\land} (x \rfrOLD{\lor} \rfrOLD{\lnot} x) = (x \rfrOLD{\land} A) \rfrOLD{\lor} (\rfrOLD{\lnot} x \rfrOLD{\land} A)) \cusand \cusand
\m \thmlink{THM-LAsc-9}{THM-LAsc-24} ((x \rfrOLD{\land} A) \rfrOLD{\lor} (\rfrOLD{\lnot} x \rfrOLD{\land} A) = (x \rfrOLD{\land} B) \rfrOLD{\lor} (\rfrOLD{\lnot} x \rfrOLD{\land} A)) \cusand \cusand
\m \thmlink{THM-LAsc-20}{THM-LAsc-25} ((x \rfrOLD{\land} B) \rfrOLD{\lor} (\rfrOLD{\lnot} x \rfrOLD{\land} A) = (x \rfrOLD{\land} B) \rfrOLD{\lor} (\rfrOLD{\lnot} x \rfrOLD{\land} B)) \cusand \cusand
\m \thmlink{POS-LDis}{THM-LAsc-26} ((x \rfrOLD{\land} B) \rfrOLD{\lor} (\rfrOLD{\lnot} x \rfrOLD{\land} B) = B \rfrOLD{\land} (x \rfrOLD{\lor} \rfrOLD{\lnot} x)) \cusand \cusand
\m \thmlink{POS-LCmp}{THM-LAsc-27} (B \rfrOLD{\land} (x \rfrOLD{\lor} \rfrOLD{\lnot} x) = B \rfrOLD{\land} \rfrOLD{T}) \cusand \cusand
\m \thmlink{POS-LIdn}{THM-LAsc-27} (B \rfrOLD{\land} \rfrOLD{T} = B) \cusand \cusand
\m \thmlink{THM-LAsc-21, THM-LAsc-22, THM-LAsc-23, THM-LAsc-24, THM-LAsc-25, THM-LAsc-26, THM-LAsc-27}{THM-LAsc-28} (A = B) \cusand \cusand
\m \thmlink{THM-LAsc-28, THM-LAsc-1}{THM-LAsc-29} (x \rfrOLD{\lor} (y \rfrOLD{\lor} z) = (x \rfrOLD{\lor} y) \rfrOLD{\lor} z) \cuspop \cusand
\m \thmlink{THM-LAsc-29, THM-Dual}{THM-LAsc} ((x \rfrOLD{\lor} (y \rfrOLD{\lor} z) = (x \rfrOLD{\lor} y) \rfrOLD{\lor} z) \cusand (x \rfrOLD{\land} (y \rfrOLD{\land} z) = (x \rfrOLD{\land} y) \rfrOLD{\land} z)) \cuspop \cuspop
\m \eqComment{Associative}
\n \thmlink{POS-LDis}{THM-LDMr-1} ((x \rfrOLD{\lor} y) \rfrOLD{\lor} (\rfrOLD{\lnot} x \rfrOLD{\land} \rfrOLD{\lnot} y) = ((x \rfrOLD{\lor} y) \rfrOLD{\lor} \rfrOLD{\lnot} x) \rfrOLD{\land} ((x \rfrOLD{\lor} y) \rfrOLD{\lor} \rfrOLD{\lnot} y)) \cusand
\m \thmlink{POS-LCom, THM-LAsc}{THM-LDMr-2} (((x \rfrOLD{\lor} y) \rfrOLD{\lor} \rfrOLD{\lnot} x) \rfrOLD{\land} ((x \rfrOLD{\lor} y) \rfrOLD{\lor} \rfrOLD{\lnot} y) = ((x \rfrOLD{\lor} \rfrOLD{\lnot} x) \rfrOLD{\lor} y) \rfrOLD{\land} ((\rfrOLD{\lnot} y \rfrOLD{\lor} y) \rfrOLD{\lor} x)) \cusand
\m \thmlink{POS-LCmp}{THM-LDMr-3} (((x \rfrOLD{\lor} \rfrOLD{\lnot} x) \rfrOLD{\lor} y) \rfrOLD{\land} ((\rfrOLD{\lnot} y \rfrOLD{\lor} y) \rfrOLD{\lor} x) = (\rfrOLD{T} \rfrOLD{\lor} y) \rfrOLD{\land} (\rfrOLD{T} \rfrOLD{\lor} x)) \cusand
\m \thmlink{THM-LDom}{THM-LDMr-4} ((\rfrOLD{T} \rfrOLD{\lor} y) \rfrOLD{\land} (\rfrOLD{T} \rfrOLD{\lor} x) = \rfrOLD{T} \rfrOLD{\land} \rfrOLD{T}) \cusand
\m \thmlink{THM-LIdm}{THM-LDMr-5} (\rfrOLD{T} \rfrOLD{\land} \rfrOLD{T} = \rfrOLD{T}) \cusand
\m \thmlink{THM-LDMr-1, THM-LDMr-2, THM-LDMr-3, THM-LDMr-4, THM-LDMr-5}{THM-LDMr-6} ((x \rfrOLD{\lor} y) \rfrOLD{\lor} (\rfrOLD{\lnot} x \rfrOLD{\land} \rfrOLD{\lnot} y) = \rfrOLD{T}) \cuspop
\m \thmlink{THM-LDis}{THM-LDMr-7} ((x \rfrOLD{\lor} y) \rfrOLD{\land} (\rfrOLD{\lnot} x \rfrOLD{\land} \rfrOLD{\lnot} y) = (x \rfrOLD{\land} \rfrOLD{\lnot} x \rfrOLD{\land} \rfrOLD{\lnot} y) \rfrOLD{\lor} (y \rfrOLD{\land} \rfrOLD{\lnot} x \rfrOLD{\land} \rfrOLD{\lnot} y)) \cusand
\m \thmlink{POS-LCom, THM-LAsc}{THM-LDMr-8} ((x \rfrOLD{\land} \rfrOLD{\lnot} x \rfrOLD{\land} \rfrOLD{\lnot} y) \rfrOLD{\lor} (y \rfrOLD{\land} \rfrOLD{\lnot} x \rfrOLD{\land} \rfrOLD{\lnot} y) = ((x \rfrOLD{\land} \rfrOLD{\lnot} x) \rfrOLD{\land} \rfrOLD{\lnot} y) \rfrOLD{\lor} ((y \rfrOLD{\land} \rfrOLD{\lnot} y) \rfrOLD{\land} \rfrOLD{\lnot} x)) \cusand
\m \thmlink{POS-LCmp}{THM-LDMr-9} (((x \rfrOLD{\land} \rfrOLD{\lnot} x) \rfrOLD{\land} \rfrOLD{\lnot} y) \rfrOLD{\lor} ((y \rfrOLD{\land} \rfrOLD{\lnot} y) \rfrOLD{\land} \rfrOLD{\lnot} x) = (\rfrOLD{F} \rfrOLD{\land} \rfrOLD{\lnot} y) \rfrOLD{\lor} (\rfrOLD{F} \rfrOLD{\land} \rfrOLD{\lnot} x)) \cusand
\m \thmlink{THM-LDom}{THM-LDMr-10} ((\rfrOLD{F} \rfrOLD{\land} \rfrOLD{\lnot} y) \rfrOLD{\lor} (\rfrOLD{F} \rfrOLD{\land} \rfrOLD{\lnot} x) = \rfrOLD{F} \rfrOLD{\lor} \rfrOLD{F}) \cusand
\m \thmlink{THM-LIdm}{THM-LDMr-11} (\rfrOLD{F} \rfrOLD{\lor} \rfrOLD{F} = \rfrOLD{F}) \cusand
\m \thmlink{THM-LDMr-7, THM-LDMr-8, THM-LDMr-9, THM-LDMr-10, THM-LDMr-11}{THM-LDMr-12} ((x \rfrOLD{\lor} y) \rfrOLD{\land} (\rfrOLD{\lnot} x \rfrOLD{\land} \rfrOLD{\lnot} y) = \rfrOLD{F}) \cuspop
\m \thmlink{THM-LDMr-6, THM-LDMr-12, POS-LCmp}{THM-LDMr-13} (((x \rfrOLD{\lor} y) \rfrOLD{\lor} (\rfrOLD{\lnot} x \rfrOLD{\land} \rfrOLD{\lnot} y) = \rfrOLD{T} = (x \rfrOLD{\lor} y) \rfrOLD{\lor} \rfrOLD{\lnot} (x \rfrOLD{\lor} y)) \cusand ((x \rfrOLD{\lor} y) \rfrOLD{\land} (\rfrOLD{\lnot} x \rfrOLD{\land} \rfrOLD{\lnot} y) = \rfrOLD{F} = (x \rfrOLD{\lor} y) \rfrOLD{\land} \rfrOLD{\lnot} (x \rfrOLD{\lor} y))) \cusand
\m \thmlink{THM-LDMr-13, THM-LUNt}{THM-LDMr-14} (\rfrOLD{\lnot} x \rfrOLD{\land} \rfrOLD{\lnot} y = \rfrOLD{\lnot} (x \rfrOLD{\lor} y)) \cusand
\m \thmlink{THM-LDMr-14, THM-Dual}{THM-LDMr} ((\rfrOLD{\lnot} x \rfrOLD{\land} \rfrOLD{\lnot} y = \rfrOLD{\lnot} (x \rfrOLD{\lor} y)) \cusand (\rfrOLD{\lnot} x \rfrOLD{\lor} \rfrOLD{\lnot} y = \rfrOLD{\lnot} (x \rfrOLD{\land} y))) \cuspop
\m \eqComment{Boolean De Morgan's Laws}
\n \thmlink{\implies}{THM-CtrP-1} (x \rfrOLD{\implies} y = (\rfrOLD{\lnot} x) \rfrOLD{\lor} y) \cusand 
\m \thmlink{POS-LCom, THM-LInv}{THM-CtrP-2} ((\rfrOLD{\lnot} x) \rfrOLD{\lor} y = ((\rfrOLD{\lnot} \rfrOLD{\lnot} y) \rfrOLD{\lor} (\rfrOLD{\lnot} x))) \cusand 
\m \thmlink{\implies}{THM-CtrP-3} ((\rfrOLD{\lnot} \rfrOLD{\lnot} y) \rfrOLD{\lor} (\rfrOLD{\lnot} x) = (\rfrOLD{\lnot} y) \rfrOLD{\implies} (\rfrOLD{\lnot} x)) \cusand 
\m \thmlink{THM-CtrP-1, THM-CtrP-2, THM-CtrP-3}{THM-CtrP} (x \rfrOLD{\implies} y = (\rfrOLD{\lnot} y) \rfrOLD{\implies} (\rfrOLD{\lnot} x)) \cuspop
\m \eqComment{Contrapositive Law} 
% http://www.cs.um.edu.mt/gordon.pace/Teaching/DiscreteMaths/Laws.pdf
\n \tdb{(\rfrOLD{T} \rfrOLD{\implies} x = x)}
\n \tdb{(\rfrOLD{F} \rfrOLD{\implies} x = \rfrOLD{T})}
\n \tdb{(x \rfrOLD{\implies} \rfrOLD{T} = \rfrOLD{T})}
\n \tdb{(x \rfrOLD{\implies} \rfrOLD{F} = \rfrOLD{\lnot} x)}  
\n \tdb{((x \rfrOLD{\lor} y) \rfrOLD{\implies} z) = (x \rfrOLD{\implies} z) \rfrOLD{\land} (y \rfrOLD{\implies} z)}
\n \tdb{(x \rfrOLD{\implies} (y \rfrOLD{\land} z) = (x \rfrOLD{\implies} y) \rfrOLD{\land} (x \rfrOLD{\implies} z))} 
\end{align}
\end{tcolorbox}

\subsection{Predicate Logic}
\begin{tcolorbox}[breakable, enhanced]
\begin{align}
\forall_{x \in \mathbb{N}} (2x/2 = x)
\n P(x) \implies D
\end{align}
\end{tcolorbox}

\end{comment}

%\section{Glossary}
%\begin{multicols}{4}
%\features
%\end{multicols}

%\bibliography{sample}

\end{document}
